Added more wp laws

theories/alpha/utp_alpha_wp.thy
@@ -9,12 +9,47 @@ ML {*
 
 setup wp.setup
 
-definition alpha_wp :: 
+definition WeakPrecondA :: 
   "'VALUE WF_ALPHA_PREDICATE \<Rightarrow> 'VALUE WF_ALPHA_PREDICATE \<Rightarrow> 'VALUE WF_ALPHA_PREDICATE" (infixr "wp" 150) where
 "Q wp r \<equiv> \<not>\<alpha> (Q ;\<alpha> (\<not>\<alpha> r))"
 
+declare WeakPrecondA_def [evala]
+
+lemma WeakPrecondA_alphabet [alphabet]:
+  "\<lbrakk> Q \<in> WF_RELATION; r \<in> WF_RELATION \<rbrakk> \<Longrightarrow>
+  \<alpha> (Q wp r) = in\<^sub>\<alpha> (\<alpha> Q) \<union>\<^sub>f out\<^sub>\<alpha> (\<alpha> r)"
+  by (simp add:WeakPrecondA_def alphabet closure)
+
+syntax
+  "_uapred_wp" :: "uapred \<Rightarrow> uapred \<Rightarrow> uapred" (infixr "wp" 55)
+
+translations
+  "_uapred_wp p q"     => "CONST WeakPrecondA p q"
+
+lemma wp_conj [wp]:
+  "\<lbrakk> P \<in> WF_RELATION; q \<in> WF_RELATION; r \<in> WF_RELATION \<rbrakk> \<Longrightarrow>
+   `P wp (q \<and> r)` = `P wp q \<and> P wp r`"
+  by (smt NotA_WF_RELATION SemiA_OrA_distl WeakPrecondA_def demorgan1 demorgan2)
+
 lemma SemiA_wp [wp]: 
-  "\<lbrakk> P \<in> WF_RELATION; Q \<in> WF_RELATION; r \<in> WF_RELATION \<rbrakk> \<Longrightarrow> (P ;\<alpha> Q) wp r = (P wp (Q wp r))"
-  by (simp add: alpha_wp_def, smt NotA_WF_RELATION SemiA_assoc)
+  "\<lbrakk> P \<in> WF_RELATION; Q \<in> WF_RELATION; r \<in> WF_RELATION \<rbrakk> 
+   \<Longrightarrow> `(P ; Q) wp r` = `P wp (Q wp r)`"
+  apply (simp add: WeakPrecondA_def)
+  apply (smt NotA_WF_RELATION SemiA_assoc)
+done
+
+lemma CondA_wp [wp]:
+  "\<lbrakk> P \<in> WF_RELATION; Q \<in> WF_RELATION; b \<in> WF_CONDITION; r \<in> WF_RELATION
+   ; \<alpha> P = \<alpha> Q; \<alpha> Q = \<alpha> r; \<alpha> b \<subseteq>\<^sub>f \<alpha> P \<rbrakk> \<Longrightarrow>
+   `(P \<triangleleft> b \<triangleright> Q) wp r` = `(P wp r) \<triangleleft> b \<triangleright> (Q wp r)`"
+  apply (simp add: WeakPrecondA_def SemiA_CondA_distr alphabet closure)
+  apply (utp_alpha_tac)
+  apply (utp_pred_auto_tac)
+done
+
+lemma OrA_wp [wp]:
+  "\<lbrakk> P \<in> WF_RELATION; Q \<in> WF_RELATION; r \<in> WF_RELATION \<rbrakk>
+   \<Longrightarrow> `(P \<or> Q) wp r` = `(P wp r) \<and> (Q wp r)`"
+  by (smt NotA_WF_RELATION SemiA_OrA_distr WeakPrecondA_def demorgan1)
 
 end
